Common/Notation.lean
@@ -6,9 +6,9 @@ class HasSubst (α : Sort _) (β : Sort _) where
 notation:200 "[" v:200 " := " w:200 "]" t:200 => HasSubst.subst v w t
 
 class HasOpen (α : Sort _) where
-  opn : Nat -> Name -> α -> α
+  opn : Nat -> α -> α -> α
 notation:200 "{" i:200 " |-> " v:200 "}" t:200 => HasOpen.opn i v t
 
 class HasClose (α : Sort _) where
-  cls : Nat -> Name -> α -> α
+  cls : α -> Name -> α -> α
 notation:200 "{" i:200 " <-| " v:200 "}" t:200 => HasClose.cls i v t
